*11612733 杜子豪*

* **1.A——**

* 2.

  $(\frac{-1+\sqrt{3}i}{2})^3=\frac{1}{8}(\sqrt{3}i-1)^2(\sqrt3i-1)$
  $=-\frac{1}{4}(\sqrt{3}i+1)(\sqrt{3}i-1)=-\frac{1}{4}[(\sqrt{3}i)^2-1]=1$

  Hence, $\frac{-1+\sqrt{3}i}{2}$ is a cube root of 1

  

* 3.

  Suppose $x=a+bi$, where $a,b\in\R$

  $x^3=i\Rightarrow(a+bi)^2=i\Rightarrow(a^2-b^2)+2abi=i$

  It follows that $a^2=b^2,2ab=1$

  Hence $b=\frac{\sqrt{2}}{2}$, $a=\pm b$

  Two square roots of $i$ are $\frac{\sqrt{2}(1+i)}{2}$ and $-\frac{\sqrt{2}(1+i)}{2}$

  

* 7.

  Since $\alpha\in\C​$, we can write $\alpha​$ as $a+bi​$ where $a,b\in\R​$

  Suppose $\beta\in\C​$, and $\beta=c+di​$ where $c,d\in\R​$

  Assume $\alpha+\beta=0$, we can get $c=-a$ and $b=-d$ which implies that there exists the unique $\beta$ s.t. $\alpha+\beta=0​$

  

* 8.

  Since $\alpha\in\C$, we can write $\alpha$ as $a+bi$ where $a,b\in\R$

  Suppose $\beta\in\C$, and $\beta=c+di$ where $c,d\in\R$

  $\alpha\beta=1\Leftrightarrow(ac-bd)+(ad+bc)i=1\Leftrightarrow ac-bd=1\;and\;ad+bc=0\Leftrightarrow c=\frac{a}{a^2+b^2}\;and\;d=-\frac{b}{a^2+b^2}$

  

* 9.

  Suppose $\lambda=m+ni$, $\alpha=a+bi$, $\beta=c+di$

  $\lambda(\alpha+\beta)=(m+ni)[(a+bi)+(c+di)]=(m+ni)(a+bi)+(m+ni)(c+di)=\lambda\alpha+\lambda\beta$

  

* 11.

  Suppose $\lambda=a+bi$

  Since $(a+bi)(2-3i)=12-5i$

  Thus $2a+3b=12$, $3a-2b=5$. Hence $a=3$, $b=2$, $\lambda=3+2i$

  However $(3+2i)(-6+7i)=-32+9i\not=-32+9i$

  Hence there does not exist such $\lambda$

  

* **1.B——**

* 1.

  $-(-v)$ is an additive inverse of $-v$

  $v$ is also an additive inverse of $-v$ 

  Since additive inverse is unique, we can get $-(-v)=v$

  

* 2

  If $a\not=0$, $\exists\;b\in\mathrm{F}$ s.t. $ab=1$

  $v=1\cdot v=(ab)v=b(av)=b\cdot0=0$

  If $a=0$, which satisfies the condition as desire.

  

* 3.

  $v+3x=w\Rightarrow x=\frac{v-w}{3}$ which proves the existance

  Suppose $y\in V$ and $y\not=x$ s.t. $v+3y=w$

  $w-w=0=3(x-y)\Rightarrow x=y$.

  Thus $x$ is unique

  

* 5.

  $v+(-1)v=[1+(-1)]v=0v=0$

  Thus they are equivalent

  

* 6.

  No. It is not a vector space, since $[+\infty+(-\infty)]+1=1$, $-\infty+[(-\infty)+1]=0$

  

* **1.C——**

* 1.

  * a.

    Assume $x_{11}+2x_{21}+3x_{31}=0$, $x_{12}+2x_{22}+3x_{32}=0​$

    $x_1=(x_{11},x_{21},x_{31})​$, $x_2=(x_{12},x_{22},x_{32})​$

    Addition:

    ​	$x_1+x_2=(x_{11}+x_{12},x_{21}+x_{22},x_{31}+x_{32})$

    ​	$(x_{11}+x_{12})+2(x_{21}+x_{22})+3(x_{31}+x_{32})=0​$

    ​	Hence, it is closed under addition

    Scalar Multiplication:

    ​	$\lambda x_1=(\lambda x_{11},\lambda x_{21},\lambda x_{31})$

    ​	$\lambda x_{11}+2(\lambda x_{21})+3(\lambda x_{31})=0​$

    ​	Hence, it is closed under scalar multiplication

    Hence it is subspace of $\mathrm{F}^3​$

  * b.

    Assume $x_{11}+2x_{21}+3x_{31}=0$, $x_{12}+2x_{22}+3x_{32}=0$

    $x_1=(x_{11},x_{21},x_{31})​$, $x_2=(x_{12},x_{22},x_{32})​$

    Addition:

    ​	$x_1+x_2=(x_{11}+x_{12},x_{21}+x_{22},x_{31}+x_{32})​$

    ​	$(x_{11}+x_{12})+2(x_{21}+x_{22})+3(x_{31}+x_{32})=8$

    ​	Hence, it is not closed under addition

    Hence it is not a subspace of $\mathrm{F}^3​$

  * c.

    Assume $V=\{(x_1,x_2,x_3)\in\mathrm{F}^3:x_1x_2x_3=0\}$

    $(1,0,0)\in V$ and $(0,1,1)\in V$

    $(1,0,0)+(0,1,1)=(1,1,1)\notin V$

    Hence it is not closed under addition.

    It is not a subspace of $\mathrm{F}^3$

  * d.

    Assume $x_{11}=5x_{31}$, $x_{12}=5x_{32}$

    $x_1=(x_{11},x_{21},x_{31})​$, $x_2=(x_{12},x_{22},x_{32})​$

    Addition:

    ​	$x_1+x_2=(x_{11}+x_{12},x_{21}+x_{22},x_{31}+x_{32})$

    ​	$(x_{11}+x_{12})=5(x_{31}+x_{32})$

    ​	Hence, it is closed under addition

    Scalar Multiplication:

    ​	$\lambda x_1=(\lambda x_{11},\lambda x_{21},\lambda x_{31})​$

    ​	$\lambda x_{11}=5(\lambda x_{31})$

    ​	Hence, it is closed under scalar multiplication

    Hence it is subspace of $\mathrm{F}^3​$

* 2.

  * a.

    Assume $x_{31}=5x_{41}+b$, $x_{32}=5x_{42}+b$

    $x_1=(x_{11},x_{21},x_{31},x_{31})​$, $x_2=(x_{12},x_{22},x_{32},x_{42})​$

    Addition:

    ​	$x_1+x_2=(x_{11}+x_{12},x_{21}+x_{22},x_{31}+x_{32},x_{41}+x_{42})$

    ​	$(x_{31}+x_{22})=5(x_{41}+x_{42})+2b$

    ​	Hence, it is closed under addition iff $2b=0\Leftrightarrow b=0$

    Scalar Multiplication:

    ​	$\lambda x_1=(\lambda x_{11},\lambda x_{21},\lambda x_{31})$

    ​	$\lambda x_{11}=5(\lambda x_{31})+b​$

    ​	Hence, it is closed under scalar multiplication iff $\lambda b\equiv0\Leftrightarrow b=0$

    Hence it is subspace of $\mathrm{F}^3$ iff $b=0$

  * b.

    Assume $f_1: [0,1]\to\R$, $f_2: [0,1]\to\R$

    Addition:

    ​	$(f_1+f_2)(x)=f_1(x)+f_2(x)$

    ​	Thus $f_1+f_2:[0,1]\to\R$

    ​	Hence it is closed under addition

    Scalar Multiplication:

    ​	$(\lambda f_1)(x)=\lambda f_1(x)$

    ​	Thus $\lambda f_1:[0,1]\to\R$

    ​	Hence it is close under scalar multiplication

    Hence it is a subspace of $\R^{[0,1]}​$

  * c.

    Assume $f_1: \R\to\R$, $f_2: \R\to\R$ 

    s.t. $f_1'​$ and $f_2'​$ exists

    Addition:

    ​	$(f_1+f_2)'(x)=f_1'(x)+f_2'(x)​$

    ​	Hence it is closed under addition

    Scalar Multiplication:

    ​	$(\lambda f_1)'(x)=\lambda f_1'(x)$

    ​	Thus $\lambda f_1:[0,1]\to\R$

    ​	Hence it is close under scalar multiplication

    Hence it is a subspace of $\R^\R{}​$

  * d.

    Assume $f_1: (0,3)\to\R$, $f_2: (0,3)\to\R$

    s.t. $f_1'(2)=f_2'(2)=b$

    Addition:

    ​	$(f_1+f_2)'(2)=f_1'(2)+f_2'(2)=2b$

    ​	Hence it is closed under addition iff $b=0$

    Scalar Multiplication:

    ​	$(\lambda f_1)'(2)=\lambda f_1'(2)=\lambda b​$

    ​	Hence it is close under scalar multiplication iff $\lambda b\equiv0\Leftrightarrow b=0$

    Hence it is a subspace of $\R^{(0,3)}$ iff $b=0$

    

* 6.

  * a.

    In $\R$, $a^3=b^3\Leftrightarrow a=b$

    Thus $\{(a,b,c)\in\R^3:a^3=b^3\}=\{(a,b,c)\in\R^3:a=b\}$

    Which is a subspace of $\R^3$

  * b.

    Let $x^3=1$, we can get $x_1=1$, $x_2=\frac{-1+\sqrt{3}i}{2}$, $x_3=\frac{-1-\sqrt{3}i}{2}$

    Assume $\alpha=(x_1,x_2,0)$, $\beta=(x_1,x_3,0)$

    $\alpha+\beta=(2,-1,0)$ where $2^3\not=(-1)^3$

    Hence it is not a subspace of $\R^3$

    

* 7.

  Let $U=\{(x,y):x,y\in\Q\}$

  Since addition in $\Q$ is closed and $\{0\}\in\Q$ Hence, $-u\in U$ whenver $u\in U$

  But if $\lambda=\pi$, $(1,1)\in U$, $\pi(1,1)\notin U$

  Hence $U$ is not a subspace of $\R^2$

  

* 8.

  Let $U=\{(x,y):x=0\;or\;y=0\}$

  Thus $\lambda(x,y)\in U$

  However, $(1,0)\in U$ and $(0,1)\in U$, $(1,0)+(0,1)=(1,1)\notin U$

  Hence $U$ is not a subspace of $\R^2$

  

* 10.

  Suppose $\forall x,y\in U_1\cap U_2$

  Thus $x+y\in U_1$ and $x+y\in U_2$, $x+y\in U_1\cap U_2$

  $\lambda x\in U_1$ and $\lambda x\in U_2$, Thus $\lambda x\in U_1\cap U_2$

  Hence $U_1\cap U_2$ is a subspace of $V$

  

* 19.

  Counterexample:

  ​	Suppose $U_1=\{(x,y)\in\R^2\}​$, $U_2=\{(x,0)\in\R^2\}​$, $W=\{(0,y)\in\R^2\}​$

  ​	$U_1+W=R^2=U_2+W$ but $U_1\not=U_2$

  

* 21.

  $W=\{(0,0,\alpha,\beta,\gamma)\in\mathrm{F}^5\}​$

* 

* 22.

  $W_1=\{(0,0,\alpha,0,0)\in\mathrm{F}^5\}$

  $W_2=\{(0,0,0,\beta,0)\in\mathrm{F}^5\}$

  $W_3=\{(0,0,0,0,\gamma)\in\mathrm{F}^5\}​$

  

* 23.

  Counterexample:

  ​	Suppose $U_1=\{(x,0)\in\R^2\}$, $U_2=\{(0,y)\in\R^2\}$, $W=\{(\alpha,\alpha)\in\R^2\}$

  ​	$U_1+W=R^2=U_2+W$ and $U_1\cap W=(0,0)=U_2\cap W$

  ​	However, $U_1\not=U_2$

  

* 24.

  If a function is odd and even, $f(x)=-f(x)\Rightarrow f(x)\equiv0$

  Thus $U_e\cap U_o=\{f:f\equiv0\}​$

  For $\forall f\in\R$, constract $g(x)=\frac{f(x)+f(-x)}{2}$ and $h(x)=\frac{f(x)-f(-x)}{2}$

  It is easy to know that $g(x)$ is even and $h(x)$ is odd

  And $f(x)=g(x)+h(x)$

  Thus $U_e+U_o=\R^{\R}$

  Hence $\R^{\R}=U_e\oplus U_o$

  

